Execution_resources/select_correctness.v
@@ -6,12 +6,6 @@ From Views.Execution_resources Require Import correctness_lemmas.
 From Views.Execution_resources Require Import sets_of_threads.
 Require Import PeanoNat.
 
-Fixpoint select_no_error (e : execution_resource) (l r : nat) (d : dimension): Prop :=
-  match e with
-  | Collection n v => forall i, i < n -> (select_no_error (v i) l r d)
-  | _ => select_range e l r d <> Error
-end.
-
 
 Proposition induction_step_collection_select :
   forall i n v m m' d l r,
@@ -41,9 +35,38 @@ Proof.
   apply le_n. apply H0.
 Qed.
 
+
+Proposition induction_step_collection_select_physical :
+  forall i n v m m' d l r f,
+(forall n' n0 n0', n' < n -> count i (physical_thread_set (v n') f) n0 ->
+    count i (physical_thread_set (select_range (v n') l r d) f) n0' -> n0' <= n0) ->
+  count i (zip (buildList n (fun i : nat => physical_thread_set (v i) f))) m
+-> count i (zip (buildList n (fun i0 : nat => physical_thread_set (select_range (v i0) l r d) f))) m'
+-> m' <= m.
+Proof.
+  induction n.
+  + intros. inversion H1. apply le_0_n.
+  + intros. simpl in *.
+  apply cat_count_rev in H0.
+  apply cat_count_rev in H1.
+  destruct H1 as [m1' [m2' [H0' [H1' H2']]]]. subst.
+  destruct H0 as [m1 [m2 [H0 [H1 H2]]]]. subst.
+  assert (forall n' n0 n0' : nat,
+    n' < n ->
+    count i (physical_thread_set (v n') f) n0 ->
+    count i (physical_thread_set (select_range (v n') l r d) f) n0' -> n0' <= n0).
+    intros. apply le_S in H2. apply H with (n0 := n0) (n0' := n0')in H2.
+    apply H2. apply H3. apply H4.
+  apply H with (n0 := m1) in H0'.
+  apply IHn with (m := m2) (m' := m2') (l := l) (r := r) (d := d) in H2.
+  apply Nat.add_le_mono. apply H0'. apply H2.
+  apply H1. apply H1'.
+  apply le_n. apply H0.
+Qed.
+
 Proposition select_correct :
   forall i e d m m' l r,
-  select_no_error e l r d -> count i (thread_set' e) m -> count i (thread_set' (select_range e l r d)) m' -> m' <= m
+  no_error e (fun e => select_range e l r d) -> count i (thread_set' e) m -> count i (thread_set' (select_range e l r d)) m' -> m' <= m
 .
 Proof.
   induction e;intros; try (exfalso; apply H; reflexivity).
@@ -180,5 +203,88 @@ Proof.
         * intros. destruct b. inversion H. simpl. apply le_S_n in H. apply IHa in H. apply H.
     } apply H1 in H0. rewrite E in H0. inversion H0.
   - right. right. right. right. right. left. reflexivity.
+Qed.
+
+Proposition select_correct_physical :
+  forall i e d m m' l r f,
+  no_error e (fun e => select_range e l r d) -> count i (physical_thread_set e f) m -> count i (physical_thread_set (select_range e l r d) f) m' -> m' <= m
+.
+Proof.
+  induction e;intros; try (exfalso; apply H; reflexivity).
+  - simpl in *. apply induction_step_collection_select_physical with (f := f) (i := i) (v := content) (n := n) (m := m) (m' := m') (l := l) (r := r) (d := d).
+    intros. apply H with (l := l) (n := n') (d := d) (r := r) (f := f). apply H0. apply H3. apply H4.
+    apply H5. apply H1. apply H2.
+  - destruct d.
+    + simpl in *. destruct (r <=? x) eqn:E.
+      ++ simpl in *. apply leb_correct in E.
+      apply zip_buildlist_inclusion with (f := (fun i : nat =>
+              zip
+                (buildList y
+                   (fun j : nat =>
+                    zip (buildList z (fun k : nat => physical_thread_set (content i j k) f)))) ++ []))
+        (a := l) (m := m) (m' := m') (i := i)
+      in E.
+      apply E. apply H2.
+      clear H2. clear E. clear H0. clear H.
+      generalize dependent m. induction x.
+      * intros. apply H1.
+      * intros. simpl in *. rewrite cat_empty. apply cat_count_rev in H1.
+      destruct H1 as [m1 [m2 [H1 [H2 H3]]]]; subst.
+      apply cat_count. apply H1. apply IHx. apply H2.
+      ++ simpl in *. exfalso. apply H0. reflexivity.
+    + simpl in *. destruct (r <=? y) eqn:E.
+      ++ simpl in *. apply leb_correct in E.
+      apply zip_buildlist_inclusion with (f := (fun i : nat =>
+              zip
+                (buildList x
+                   (fun i0 : nat =>
+                    zip (buildList z (fun k : nat => physical_thread_set (content i0 i k) f)) ++ []))))
+        (a := l) (m := m) (m' := m') (i := i)
+      in E.
+      apply E. apply H2.
+      apply transpose_lemma.
+      clear H2. clear E. clear H0. clear H.
+      generalize dependent m. induction x.
+      * intros. apply H1.
+      * intros. simpl in *. apply cat_count_rev in H1.
+      destruct H1 as [m1 [m2 [H1 [H2 H3]]]]; subst.
+      apply cat_count. clear H2. clear IHx.
+        generalize dependent m1. induction y. intros.
+            apply H1. intros. apply cat_count_rev in H1.
+        destruct H1 as [m1' [m2' [H1 [H2 H3]]]]; subst.
+        apply cat_count. rewrite cat_empty. apply H1. apply IHy.
+        apply H2.
+      apply IHx. apply H2.
+      ++ simpl in *. exfalso. apply H0. reflexivity.
+    + simpl in *. destruct (r <=? z) eqn:E.
+      ++ simpl in *. apply leb_correct in E.
+      apply zip_buildlist_inclusion with (f := (fun i : nat =>
+              zip
+                (buildList x
+                   (fun i0 : nat =>
+                    zip (buildList y (fun j : nat => physical_thread_set (content i0 j i) f ++ []))))))
+        (a := l) (m := m) (m' := m') (i := i)
+      in E.
+      apply E. apply H2.
+      apply transpose_lemma.
+      apply transpose_lemma'.
+      clear H2. clear E. clear H0. clear H.
+      generalize dependent m. induction x.
+      * intros. apply H1.
+      * intros. simpl in *. apply cat_count_rev in H1.
+      destruct H1 as [m1 [m2 [H1 [H2 H3]]]]; subst.
+      apply cat_count. clear H2. clear IHx.
+        generalize dependent m1. induction y. intros.
+          apply H1. intros. apply cat_count_rev in H1.
+          destruct H1 as [m1' [m2' [H1 [H2 H3]]]]; subst.
+          apply cat_count. clear H2. clear IHy.
+          generalize dependent m1'. induction z. intros.
+            apply H1. intros. apply cat_count_rev in H1.
+            destruct H1 as [m1'' [m2'' [H1 [H2 H3]]]]; subst.
+            apply cat_count. rewrite cat_empty. apply H1. apply IHz.
+            apply H2.
+        apply IHy. apply H2.
+      apply IHx. apply H2.
+      ++ simpl in *. exfalso. apply H0. reflexivity.
 Qed.
 
